
\section{Problema 2.} Resuelva: 
$$\frac{\partial ^2 u}{\partial t^2}= a^2\frac{\partial ^2 u}{\partial x^2}, \quad 0<x<L, t>0.$$
Sujeta a: $u(0,t)=0, \frac{\partial u}{\partial x}(L,t)=K$ y con $u(x,0)=0, \frac{\partial u}{\partial t}(x,0)=0.$

\begin{solution}
\begin{align*}
	\Laplace{\frac{\partial ^2 u}{\partial t^2}} &= a^2 \Laplace{\frac{\partial ^2 u}{\partial x^2}}\\
	s^2\widehat{u}(x,s)-su(x,0)-u'(x,0) &= a^2\widehat{u}''(x,s)\\
	s^2\widehat{u}(x,s)-0- 0&= a^2\widehat{u}''(x,s)\\
	a^2\widehat{u}''(x,s)-s^2\widehat{u}(x,s)&= 0\\
	\widehat{u}''(x,s)-\left(\frac{s}{a}\right)^2\widehat{u}(x,s)&= 0
\end{align*}
La soluci贸n de la EDO:
$$\widehat{u}(x,s) = Ae^{\frac{s}{a}x}+Be^{-\frac{s}{a}x}$$
Tenemos la condici贸n $\widehat{u}(0,t)=0$:
$$\widehat{u}(0,t)=Ae^{\frac{s}{a}x}-Ae^{-\frac{s}{a}x}=A\left(e^{\frac{s}{a}x}-e^{-\frac{s}{a}x}\right)=2A\senh\left(\frac{s}{a}x\right)$$
Aplicando la condici贸n $\frac{\partial u}{\partial x }(L,t)=K$: 
\begin{align*}
	\widehat{u}'(x,t) &= A\left(\frac{s}{a}e^{\frac{s}{a}x}+\frac{s}{a}e^{-\frac{s}{a}x}\right)\\
									&= \frac{2As}{a}\cosh\left(\frac{s}{a}x\right)\\
	\widehat{u}'(L,t) &= \frac{2As}{a}\cosh\left(\frac{s}{a}L\right) =\frac{k}{s}
\end{align*}
$$A=\frac{aK}{2s^2\cosh\left(\frac{s}{a}L\right)}$$
Entonces, tenemos: 
$$\widehat{u}(x,s)=\frac{aK}{s^2\cosh\left(\frac{s}{a}L\right)}\senh\left(\frac{s}{a}x\right)$$
Entonces, la soluci贸n: 
$$u(x,t)=\iLaplace{\frac{aK\senh\left(\frac{s}{a}x\right)}{s^2\cosh\left(\frac{s}{a}L\right)}}$$

\end{solution}